semantics/prop/vyperTypeStmtSoundnessScript.sml
@@ -12,7 +12,7 @@ Ancestors
   vyperTypeEnv vyperTypeEnvPreservation vyperTypeBuiltins vyperTypeExprSoundness
   vyperStatePreservation vyperTypeStatePreservation
 Libs
-  wordsLib
+  wordsLib markerLib
 
 (* ===== Exception/result typing ===== *)
 
@@ -147,6 +147,351 @@ QED
 (* TOP-LEVEL WORKHORSE: mutual no-TypeError proof for statements, statement
  * lists, and for-loops.  This follows the evaluator recursion and is the
  * intended final shape for removing the no-TypeError cheats. *)
+Theorem eval_all_no_type_error_mutual:
+  (!cx s. !env ret_ty env' st res st'.
+    type_stmt env ret_ty s = SOME env' /\ env_consistent env cx st /\ state_well_typed st /\
+    context_well_typed cx /\ accounts_well_typed st.accounts /\ functions_well_typed cx /\
+    eval_stmt cx s st = (res, st') ==>
+    no_type_error_result res) /\
+  (!cx ss. !env ret_ty env' st res st'.
+    type_stmts env ret_ty ss = SOME env' /\ env_consistent env cx st /\ state_well_typed st /\
+    context_well_typed cx /\ accounts_well_typed st.accounts /\ functions_well_typed cx /\
+    eval_stmts cx ss st = (res, st') ==>
+    no_type_error_result res) /\
+  (!cx it. !env ty st res st'.
+    well_typed_iterator env ty it /\ env_consistent env cx st /\ state_well_typed st /\
+    context_well_typed cx /\ accounts_well_typed st.accounts /\ functions_well_typed cx /\
+    eval_iterator cx it st = (res, st') ==>
+    no_type_error_result res) /\
+  (!cx tgt. !env ty st res st'.
+    well_typed_atarget env tgt ty /\ env_consistent env cx st /\ state_well_typed st /\
+    context_well_typed cx /\ accounts_well_typed st.accounts /\ functions_well_typed cx /\
+    eval_target cx tgt st = (res, st') ==>
+    no_type_error_result res) /\
+  (!cx tgts. !env tys st res st'.
+    LIST_REL (\t ty. well_typed_atarget env t ty) tgts tys /\
+    env_consistent env cx st /\ state_well_typed st /\
+    context_well_typed cx /\ accounts_well_typed st.accounts /\ functions_well_typed cx /\
+    eval_targets cx tgts st = (res, st') ==>
+    no_type_error_result res) /\
+  (!cx bt. !env vt st res st'.
+    type_place_target env bt = SOME vt /\ env_consistent env cx st /\ state_well_typed st /\
+    context_well_typed cx /\ accounts_well_typed st.accounts /\ functions_well_typed cx /\
+    eval_base_target cx bt st = (res, st') ==>
+    no_type_error_result res) /\
+  (!cx tyv id body vs. !env ret_ty ty env_after st res st'.
+    evaluate_type env.type_defs ty = SOME tyv /\ EVERY (value_has_type tyv) vs /\
+    id NOTIN FDOM env.var_types /\
+    type_stmts (extend_local env id ty F) ret_ty body = SOME env_after /\
+    env_consistent env cx st /\ state_well_typed st /\
+    context_well_typed cx /\ accounts_well_typed st.accounts /\ functions_well_typed cx /\
+    eval_for cx tyv id body vs st = (res, st') ==>
+    no_type_error_result res) /\
+  (!cx e. !env st res st'.
+    well_typed_expr env e /\ env_consistent env cx st /\ state_well_typed st /\
+    context_well_typed cx /\ accounts_well_typed st.accounts /\ functions_well_typed cx /\
+    eval_expr cx e st = (res, st') ==>
+    no_type_error_result res) /\
+  (!cx es. !env st res st'.
+    well_typed_exprs env es /\ env_consistent env cx st /\ state_well_typed st /\
+    context_well_typed cx /\ accounts_well_typed st.accounts /\ functions_well_typed cx /\
+    eval_exprs cx es st = (res, st') ==>
+    no_type_error_result res)
+Proof
+  ho_match_mp_tac evaluate_ind >> rpt conj_tac >>
+  rpt gen_tac >> strip_tac >>
+  TRY(rename1 `Pass` >> suspend "Pass") >>
+  TRY(rename1 `Continue` >> suspend "Continue") >>
+  TRY(rename1 `Break` >> suspend "Break") >>
+  TRY(rename1 `Return NONE` >> suspend "Return_NONE") >>
+  TRY(rename1 `Return (SOME _)` >> suspend "Return_SOME") >>
+  TRY(rename1 `Raise RaiseBare` >> suspend "RaiseBare") >>
+  TRY(rename1 `Raise RaiseUnreachable` >> suspend "RaiseUnreachable") >>
+  TRY(rename1 `Raise (RaiseReason _)` >> suspend "RaiseReason") >>
+  TRY(rename1 `AssertBare` >> suspend "AssertBare") >>
+  TRY(rename1 `AssertUnreachable` >> suspend "AssertUnreachable") >>
+  TRY(rename1 `AssertReason` >> suspend "AssertReason") >>
+  TRY(rename1 `Log` >> suspend "Log") >>
+  TRY(rename1 `AnnAssign` >> suspend "AnnAssign") >>
+  TRY(rename1 `Append` >> suspend "Append") >>
+  TRY(rename1 `Assign` >> suspend "Assign") >>
+  TRY(rename1 `AugAssign` >> suspend "AugAssign") >>
+  TRY(rename1 `If` >> suspend "If") >>
+  TRY(rename1 `For` >> suspend "For") >>
+  TRY(rename1 `Expr` >> suspend "Expr") >>
+  TRY(rename1 `eval_stmts _ []` >> suspend "Stmts_nil") >>
+  TRY(rename1 `eval_stmts _ (_::_)` >> suspend "Stmts_cons") >>
+  TRY(rename1 `eval_for _ _ _ _ []` >> suspend "For_nil") >>
+  TRY(rename1 `eval_for _ _ _ _ (_::_)` >> suspend "For_cons") >>
+  TRY(rename1 `Array` >> suspend "Iterator_Array") >>
+  TRY(rename1 `Range` >> suspend "Iterator_Range") >>
+  TRY(rename1 `BaseTarget` >> suspend "Target_Base") >>
+  TRY(rename1 `TupleTarget` >> suspend "Target_Tuple") >>
+  TRY(rename1 `eval_targets _ []` >> suspend "Targets_nil") >>
+  TRY(rename1 `eval_targets _ (_::_)` >> suspend "Targets_cons") >>
+  TRY(rename1 `NameTarget` >> suspend "BaseTarget_Name") >>
+  TRY(rename1 `BareGlobalNameTarget` >> suspend "BaseTarget_BareGlobal") >>
+  TRY(rename1 `TopLevelNameTarget` >> suspend "BaseTarget_TopLevel") >>
+  TRY(rename1 `SubscriptTarget` >> suspend "BaseTarget_Subscript") >>
+  TRY(rename1 `AttributeTarget` >> suspend "BaseTarget_Attribute") >>
+  TRY(rename1 `Name` >> suspend "Expr_Name") >>
+  TRY(rename1 `BareGlobalName` >> suspend "Expr_BareGlobalName") >>
+  TRY(rename1 `TopLevelName` >> suspend "Expr_TopLevelName") >>
+  TRY(rename1 `FlagMember` >> suspend "Expr_FlagMember") >>
+  TRY(rename1 `IfExp` >> suspend "Expr_IfExp") >>
+  TRY(rename1 `Literal` >> suspend "Expr_Literal") >>
+  TRY(rename1 `StructLit` >> suspend "Expr_StructLit") >>
+  TRY(rename1 `Subscript` >> suspend "Expr_Subscript") >>
+  TRY(rename1 `Attribute` >> suspend "Expr_Attribute") >>
+  TRY(rename1 `Builtin` >> suspend "Expr_Builtin") >>
+  TRY(rename1 `TypeBuiltin` >> suspend "Expr_TypeBuiltin") >>
+  TRY(rename1 `Pop` >> suspend "Expr_Pop") >>
+  TRY(rename1 `IntCall` >> suspend "Expr_Call_IntCall") >>
+  TRY(rename1 `ExtCall` >> suspend "Expr_Call_ExtCall") >>
+  TRY(rename1 `Send` >> suspend "Expr_Call_Send") >>
+  TRY(rename1 `RawCallTarget` >> suspend "Expr_Call_RawCallTarget") >>
+  TRY(rename1 `RawLog` >> suspend "Expr_Call_RawLog") >>
+  TRY(rename1 `RawRevert` >> suspend "Expr_Call_RawRevert") >>
+  TRY(rename1 `SelfDestructTarget` >> suspend "Expr_Call_SelfDestructTarget") >>
+  TRY(rename1 `CreateTarget` >> suspend "Expr_Call_CreateTarget") >>
+  TRY(rename1 `eval_exprs _ []` >> suspend "Exprs_nil") >>
+  TRY(rename1 `eval_exprs _ (_::_)` >> suspend "Exprs_cons")
+QED
+
+Resume eval_all_no_type_error_mutual[Pass]:
+  gvs[Once evaluate_def, return_def, no_type_error_result_def]
+QED
+
+Resume eval_all_no_type_error_mutual[Continue]:
+  gvs[Once evaluate_def, raise_def, no_type_error_result_def]
+QED
+
+Resume eval_all_no_type_error_mutual[Break]:
+  gvs[Once evaluate_def, raise_def, no_type_error_result_def]
+QED
+
+Resume eval_all_no_type_error_mutual[Stmts_nil]:
+  gvs[Once evaluate_def, return_def, no_type_error_result_def]
+QED
+
+Resume eval_all_no_type_error_mutual[Return_NONE]:
+  gvs[type_stmt_def, Once evaluate_def, raise_def, no_type_error_result_def]
+QED
+
+Resume eval_all_no_type_error_mutual[Return_SOME]:
+  rpt gen_tac >> strip_tac >>
+  gvs[type_stmt_def, Once evaluate_def, bind_def, raise_def, AllCaseEqs(),
+      no_type_error_result_def] >>
+  first_x_assum drule_all >> rw[no_type_error_result_def] >>
+  rpt (BasicProvers.TOP_CASE_TAC >> gvs[no_type_error_result_def]) >>
+  drule_all eval_expr_type_preservation >> strip_tac >>
+  gvs[expr_runtime_typed_def] >>
+  drule_all evaluate_type_not_NoneT_imp_not_NoneTV >> strip_tac >>
+  drule_all materialise_typed_non_none_no_type_error >> simp[]
+QED
+
+Resume eval_all_no_type_error_mutual[RaiseBare]:
+  gvs[type_stmt_def, Once evaluate_def, raise_def, no_type_error_result_def]
+QED
+
+Resume eval_all_no_type_error_mutual[RaiseUnreachable]:
+  gvs[type_stmt_def, Once evaluate_def, raise_def, no_type_error_result_def]
+QED
+
+Resume eval_all_no_type_error_mutual[RaiseReason]:
+  cheat
+QED
+
+Resume eval_all_no_type_error_mutual[AssertBare]:
+  cheat
+QED
+
+Resume eval_all_no_type_error_mutual[AssertUnreachable]:
+  cheat
+QED
+
+Resume eval_all_no_type_error_mutual[AssertReason]:
+  cheat
+QED
+
+Resume eval_all_no_type_error_mutual[Log]:
+  cheat
+QED
+
+Resume eval_all_no_type_error_mutual[AnnAssign]:
+  cheat
+QED
+
+Resume eval_all_no_type_error_mutual[Append]:
+  cheat
+QED
+
+Resume eval_all_no_type_error_mutual[Assign]:
+  cheat
+QED
+
+Resume eval_all_no_type_error_mutual[AugAssign]:
+  cheat
+QED
+
+Resume eval_all_no_type_error_mutual[If]:
+  cheat
+QED
+
+Resume eval_all_no_type_error_mutual[For]:
+  cheat
+QED
+
+Resume eval_all_no_type_error_mutual[Expr]:
+  cheat
+QED
+
+Resume eval_all_no_type_error_mutual[Stmts_cons]:
+  cheat
+QED
+
+Resume eval_all_no_type_error_mutual[Iterator_Array]:
+  cheat
+QED
+
+Resume eval_all_no_type_error_mutual[Iterator_Range]:
+  cheat
+QED
+
+Resume eval_all_no_type_error_mutual[Target_Base]:
+  cheat
+QED
+
+Resume eval_all_no_type_error_mutual[Target_Tuple]:
+  cheat
+QED
+
+Resume eval_all_no_type_error_mutual[Targets_nil]:
+  cheat
+QED
+
+Resume eval_all_no_type_error_mutual[Targets_cons]:
+  cheat
+QED
+
+Resume eval_all_no_type_error_mutual[BaseTarget_Name]:
+  cheat
+QED
+
+Resume eval_all_no_type_error_mutual[BaseTarget_BareGlobal]:
+  cheat
+QED
+
+Resume eval_all_no_type_error_mutual[BaseTarget_TopLevel]:
+  cheat
+QED
+
+Resume eval_all_no_type_error_mutual[BaseTarget_Subscript]:
+  cheat
+QED
+
+Resume eval_all_no_type_error_mutual[BaseTarget_Attribute]:
+  cheat
+QED
+
+Resume eval_all_no_type_error_mutual[Expr_Name]:
+  cheat
+QED
+
+Resume eval_all_no_type_error_mutual[Expr_BareGlobalName]:
+  cheat
+QED
+
+Resume eval_all_no_type_error_mutual[Expr_TopLevelName]:
+  cheat
+QED
+
+Resume eval_all_no_type_error_mutual[Expr_FlagMember]:
+  cheat
+QED
+
+Resume eval_all_no_type_error_mutual[Expr_IfExp]:
+  cheat
+QED
+
+Resume eval_all_no_type_error_mutual[Expr_Literal]:
+  cheat
+QED
+
+Resume eval_all_no_type_error_mutual[Expr_StructLit]:
+  cheat
+QED
+
+Resume eval_all_no_type_error_mutual[Expr_Subscript]:
+  cheat
+QED
+
+Resume eval_all_no_type_error_mutual[Expr_Attribute]:
+  cheat
+QED
+
+Resume eval_all_no_type_error_mutual[Expr_Builtin]:
+  cheat
+QED
+
+Resume eval_all_no_type_error_mutual[Expr_TypeBuiltin]:
+  cheat
+QED
+
+Resume eval_all_no_type_error_mutual[Expr_Pop]:
+  cheat
+QED
+
+Resume eval_all_no_type_error_mutual[Expr_Call_IntCall]:
+  cheat
+QED
+
+Resume eval_all_no_type_error_mutual[Expr_Call_ExtCall]:
+  cheat
+QED
+
+Resume eval_all_no_type_error_mutual[Expr_Call_Send]:
+  cheat
+QED
+
+Resume eval_all_no_type_error_mutual[Expr_Call_RawCallTarget]:
+  cheat
+QED
+
+Resume eval_all_no_type_error_mutual[Expr_Call_RawLog]:
+  cheat
+QED
+
+Resume eval_all_no_type_error_mutual[Expr_Call_RawRevert]:
+  cheat
+QED
+
+Resume eval_all_no_type_error_mutual[Expr_Call_SelfDestructTarget]:
+  cheat
+QED
+
+Resume eval_all_no_type_error_mutual[Expr_Call_CreateTarget]:
+  cheat
+QED
+
+Resume eval_all_no_type_error_mutual[Exprs_nil]:
+  cheat
+QED
+
+Resume eval_all_no_type_error_mutual[Exprs_cons]:
+  cheat
+QED
+
+Resume eval_all_no_type_error_mutual[For_nil]:
+  gvs[Once evaluate_def, return_def, no_type_error_result_def]
+QED
+
+Resume eval_all_no_type_error_mutual[For_cons]:
+  cheat
+QED
+
+Finalise eval_all_no_type_error_mutual
+
 Theorem eval_stmt_stmts_for_no_type_error_mutual:
   (!cx s st res st' env ret_ty env'.
     type_stmt env ret_ty s = SOME env' /\ env_consistent env cx st /\ state_well_typed st /\
@@ -167,7 +512,7 @@ Theorem eval_stmt_stmts_for_no_type_error_mutual:
     eval_for cx tyv id body vs st = (res, st') ==>
     no_type_error_result res)
 Proof
-  cheat
+  metis_tac[eval_all_no_type_error_mutual]
 QED
 
 Theorem eval_stmt_no_type_error:
@@ -181,7 +526,6 @@ Proof
   irule (cj 1 eval_stmt_stmts_for_no_type_error_mutual) >>
   metis_tac[]
 QED
-
 
 Theorem eval_stmt_type_preservation_success:
   type_stmt env ret_ty s = SOME env' /\ env_consistent env cx st /\ state_well_typed st /\
